BasePrelude.v
@@ -16,7 +16,6 @@ Local Definition plus_k_index (l: list (BasicAst.context_decl nat)) k :=
 Local Definition minus_one_index (l: list (BasicAst.context_decl nat)) :=
   map (fun x => mkdeclnat x.(decl_name) x.(decl_body) (x.(decl_type)-1)) l.
 
-
 Inductive information : Type :=
 | information_list (l : list (BasicAst.context_decl nat))
 | information_nat (n : nat).
@@ -46,6 +45,22 @@ Local Fixpoint replace_add_info (info:list (string * information)) (na:string) (
   | [] => (na, information_list [item]) :: []
   end.
 
+(*find the index of [x] in the list [l]*)
+Local Definition findi (x:nat) (l:list nat):=
+  let fix Ffix x l n:=
+    match l with
+    | [] => None
+    | y :: l' => if eqb y x then Some n else Ffix x l' (n+1)
+    end
+  in
+  Ffix x l 0.
+
+(*repeat calling a function*)
+Local Fixpoint redo {A} (f:A->A) n a :=
+  match n with
+  | 0 => a
+  | S n => f (redo f n a) end.
+
 
 (****************************************************************)
 (*
@@ -53,8 +68,8 @@ Local Fixpoint replace_add_info (info:list (string * information)) (na:string) (
 
   ex.
     Inductive type ===> identity function
-    Inductive type ===> inductive principle
-    Inductive type ===> type of inductive principle
+    Inductive type ===> induction principle
+    Inductive type ===> type of induction principle
 
   Source of the generation : type definition
   Target: ......
@@ -83,16 +98,18 @@ Local Fixpoint replace_add_info (info:list (string * information)) (na:string) (
 
 *)
 Record extrainfo : Type := mkinfo {
-  renaming : list (BasicAst.context_decl nat);
+  renaming : list (BasicAst.context_decl term);
   (*info: to save some useful information (parameters, indices, ...) *)
   info : list (string * information) ;
+
+  info_source: list (string * information) ;
   kn : kername;
 }.
 
 
 
-Definition add_listinfo e na l :extrainfo :=
-  mkinfo e.(renaming) ((na, information_list l)::e.(info)) e.(kn).
+Local Definition add_listinfo e na l :extrainfo :=
+  mkinfo e.(renaming) ((na, information_list l)::e.(info)) e.(info_source) e.(kn).
 
 Definition add_info_names (e:extrainfo) (str:string) names : extrainfo :=
   let l:= mapi (fun i x => mkdeclnat x None i) names in
@@ -100,14 +117,25 @@ Definition add_info_names (e:extrainfo) (str:string) names : extrainfo :=
 
 (*Make the initial information.
   By default, we begin with the info which contains only the kername,
-  and the list of type names
-*)
+  and the list of type names *)
 Definition make_initial_info (kn:kername) (ty:mutual_inductive_body) :extrainfo :=
-  let e := mkinfo [] [] kn in
-  add_info_names e "rels_of_T"
+  let types :=
     (map (fun ind_body => {| binder_name := nNamed (ind_body.(ind_name));
                         binder_relevance := Relevant  |}
-          ) ty.(ind_bodies)).
+          ) ty.(ind_bodies))
+  in
+  let len := length types in
+  mkinfo
+    (mapi
+      (fun i x =>
+        mkdecl x None
+          (tInd
+            {| inductive_mind := kn; inductive_ind := len - i -1 |}
+            []))
+      types)
+    []
+    [("rels_of_T", information_list (mapi (fun i x => mkdeclnat x None i) types))] 
+    kn.
 
 (*The indicator which shows if some new information should be saved
   when new variable introduced *)
@@ -116,10 +144,16 @@ Inductive saveinfo:=
   | Saveitem (s:string)
   | NoSave.
 
+Local Definition lift_renaming t :=
+  map (fun t => match decl_type t with
+        | tRel i => mkdecl t.(decl_name) t.(decl_body) (tRel (i + 1))
+        | _ => t end) t.
+
 Local Definition update_kp (na:aname) (e:extrainfo) (saveinfo:saveinfo):=
   let item := mkdeclnat na None 0 in
+  let item_rename := mkdecl na None (tRel 0) in
   let renaming :=
-    item :: (plus_one_index e.(renaming))
+    item_rename :: (lift_renaming e.(renaming))
   in
   let info :=
     map (
@@ -128,59 +162,61 @@ Local Definition update_kp (na:aname) (e:extrainfo) (saveinfo:saveinfo):=
       | (na, information_nat n) => (na, information_nat (1 + n)) end
     ) e.(info)
   in
+  let info_source :=
+    map (
+      fun x => match x with
+      | (na, information_list l) => (na, information_list (plus_one_index l))
+      | (na, information_nat n) => (na, information_nat (1 + n)) end
+    ) e.(info_source)
+  in
   match saveinfo with
-  | NoSave => mkinfo renaming info e.(kn)
-  | Saveitem str => mkinfo renaming ((str, information_nat 0) ::info) e.(kn)
-  | Savelist str => mkinfo renaming (replace_add_info info str item) e.(kn)
+  | NoSave => mkinfo renaming info info_source e.(kn)
+  | Saveitem str => mkinfo renaming ((str, information_nat 0) ::info) info_source e.(kn)
+  | Savelist str => mkinfo renaming (replace_add_info info str item) info_source e.(kn)
   end
   .
 
 Local Definition update_mk na (e:extrainfo) (saveinfo:saveinfo) : extrainfo :=
   let info := map (
     fun x => match x with
-    | (na, information_list l) =>
-        if String.eqb na "rels_of_T" then x else
-        (na, information_list (plus_one_index l))
+    | (na, information_list l) => (na, information_list (plus_one_index l))
     | (na, information_nat n) => (na, information_nat (1 + n)) end
   ) e.(info) in
-  let renaming := plus_one_index e.(renaming) in
+  let renaming := lift_renaming e.(renaming) in
   let item := mkdeclnat na None 0 in
   match saveinfo with
-  | NoSave => mkinfo renaming info e.(kn)
-  | Saveitem str => mkinfo renaming ((str, information_nat 0)::info) e.(kn)
-  | Savelist str => mkinfo renaming (replace_add_info info str item) e.(kn)
+  | NoSave => mkinfo renaming info e.(info_source) e.(kn)
+  | Saveitem str => mkinfo renaming ((str, information_nat 0)::info) e.(info_source) e.(kn)
+  | Savelist str => mkinfo renaming (replace_add_info info str item) e.(info_source) e.(kn)
   end.
 
+(*return the [i]th element of the [e.(renaming)].
+  Only used in type_rename_transformor currently*)
+Local Definition geti_rename (e:extrainfo) (i:nat) :=
+  let l := map (fun x => x.(decl_type)) e.(renaming) in
+  (nth i l todo).
+
+(**************************************)
+(* this part is for "match with", already used in "generate_identity.v", with good result.
+   but maybe need to be rewritten. *)
 Local Definition add_args (e:extrainfo) (ctx: context): extrainfo :=
   let nargs := length ctx in
-  let l:= mapi (fun i x => mkdeclnat x.(decl_name) None i) (ctx) in
+  let l:= mapi (fun i x => mkdecl x.(decl_name) None (tRel i)) (ctx) in
   (*start with the last argument*)
-  let renaming := (tl l) ++ (plus_k_index e.(renaming) (nargs)) in
+  let renaming := (tl l)
+    ++ (redo lift_renaming nargs e.(renaming)) in
   let info_new := map (
     fun x => match x with
-    | (na, information_list l) =>
-        if String.eqb "rels_of_T" na  then
-          (na, information_list (plus_k_index l (nargs-1)))
-        else
-          (na, information_list (plus_k_index l nargs))
+    | (na, information_list l) => (na, information_list (plus_k_index l nargs))
     | (na, information_nat n) => (na, information_nat (n + nargs)) end
     ) e.(info) in
-  let arg := information_nat 0 in
-  mkinfo (renaming) (("arg_current", arg):: info_new) e.(kn).
-
-(* Local Definition add_args' (e:extrainfo) (ctx: context): extrainfo :=
-  let nargs := length ctx in
-  let renaming := plus_k_index e.(renaming) (nargs) in
-  let info_new := map (
+  let info_source := map (
     fun x => match x with
-    | information_list na l =>
-        if String.eqb "rels_of_T" na then x
-        else information_list na (plus_k_index l nargs)
-    | information_nat na n => information_nat na (n + nargs) end
-    ) e.(info) in
-  mkinfo renaming info_new e.(kn).
- *)
-
+    | (na, information_list l) => (na, information_list (plus_k_index l (nargs-1)))
+    | (na, information_nat n) => (na, information_nat (n + nargs)) end
+    ) e.(info_source) in
+  let arg := information_nat 0 in
+  mkinfo (renaming) (("arg_current", arg):: info_new) info_source e.(kn).
 
 Definition fancy_tCase (e:extrainfo) t0 t2 t3 t4 t5 t6 t7 (t8:extrainfo -> list (context * (extrainfo -> term))):term :=
   let pcontext := t5 e in
@@ -194,11 +230,16 @@ Definition fancy_tCase (e:extrainfo) t0 t2 t3 t4 t5 t6 t7 (t8:extrainfo -> list 
       | (na, information_list l) => (na, information_list (plus_k_index l (length pcontext)))
       | (na, information_nat n) => (na, information_nat (n + length pcontext)) end
     ) info in
+    let info_source := map (
+      fun x => match x with
+      | (na, information_list l) => (na, information_list (plus_k_index l (length pcontext)))
+      | (na, information_nat n) => (na, information_nat (n + length pcontext)) end
+    ) e.(info_source) in
     (*very limited*)
     let l:= mapi (fun i x => mkdeclnat x None (i+1)) (tl pcontext) in
-    let renaming_new := plus_k_index renaming (length pcontext) in
+    let renaming_new := redo lift_renaming (length pcontext) renaming in
     let info_new := ("pcontext_indices", information_list l) :: info_new in
-    mkinfo renaming_new info_new e.(kn)
+    mkinfo renaming_new info_new info_source e.(kn)
   in
   tCase
     {|
@@ -222,46 +263,18 @@ Definition fancy_tCase (e:extrainfo) t0 t2 t3 t4 t5 t6 t7 (t8:extrainfo -> list 
 Local Definition update_ctr_arg_back (e:extrainfo) : extrainfo :=
   let info_new := map (
     fun x => match x with
-    | (na, information_list l) =>
-        if String.eqb "rels_of_T" na then
-          (na, information_list (minus_one_index l))
-        else x
+    | (na, information_list l) => x
     | (na, information_nat n) =>
         if String.eqb "arg_current" na then (na, information_nat (n + 1))
         else x end
   ) e.(info) in
-  mkinfo (tl e.(renaming)) info_new e.(kn)
+  let info_source := map (
+    fun x => match x with
+    | (na, information_list l) => (na, information_list (minus_one_index l))
+    | (na, information_nat n) => x end
+  ) e.(info_source) in
+  mkinfo (tl e.(renaming)) info_new info_source e.(kn)
 .
-
-(* Search "length" "fold". *)
-(* Local Definition update_ctr_arg' (e:extrainfo) : extrainfo := todo
-.
-
-Definition handle_arg (arg:context_decl)
-  (f:context_decl->extrainfo->term->term)
-  (e:extrainfo) (t:extrainfo->term): term :=
-  f arg e (t (update_ctr_arg' e)).
-
-Fixpoint fold_arg {X} (args:context) (f:context_decl->extrainfo-> X -> X)
-  (e:extrainfo) (t: extrainfo -> X): X :=
-  match args with
-  | [] => t e
-  | arg :: l => f arg e (fold_arg l f (update_ctr_arg' e) t)
-  end.
-
-Definition map_with_info_arg' (f:context_decl -> extrainfo -> term)
-  (l:context) (e:extrainfo): list term:=
-  fold_arg l (
-    fun arg tl =>
-      (f arg e) :: tl
-  ) e (fun _ => []).
-
-Definition auxarg (arg:context_decl) (e:extrainfo) : term := todo.
-
-Definition testmyf (b:constructor_body) (e:extrainfo): list term :=
-  map_with_info_arg' auxarg (rev b.(cstr_args)) e.
-*)
-
 
 (*Used only when tCase, match with ..., to be explained *)
 Definition map_with_extrainfo_arg {X Y:Type} (f:X -> extrainfo -> Y) (l:list X)
@@ -273,39 +286,10 @@ Definition map_with_extrainfo_arg {X Y:Type} (f:X -> extrainfo -> Y) (l:list X)
     end
   in
   Ffix f l e.
-
-Local Definition findi (x:nat) (l:list nat):=
-  let fix Ffix x l n:=
-    match l with
-    | [] => None
-    | y :: l' => if eqb y x then Some n else Ffix x l' (n+1)
-    end
-  in
-  Ffix x l 0.
-
-(*
-  Used for lambda type argument. To be explained
-*)
-Definition check_return_type (t:term) (e:extrainfo) : option nat :=
-  let fix Ffix t e {struct t}:=
-    match t with
-    | tRel i =>
-      let types := lookup_list e.(info) "rels_of_T" in
-      let types := map decl_type types in
-      findi i types
-    | tApp t _ => Ffix t e
-    | tProd name _  t2 => Ffix t2 (update_kp name e NoSave)
-    | _ => None
-    end in
-  Ffix t e.
+(**************************************)
 
 
-
-(****************************************************************)
-(*return the tRel term of the [i]th element of the [e.(renaming)] *)
-Definition geti_rename (e:extrainfo) (i:nat) :=
-  let l := map (fun x => x.(decl_type)) e.(renaming) in
-  tRel (nth i l todo).
+(******************************  API  *******************************)
 
 (*return the tRel term of the [i]th element of the information list named [na] inside [e.(info)] *)
 Definition geti_info (na:string) (e:extrainfo) (i:nat) :=
@@ -322,6 +306,7 @@ Definition rel_of (na:string) (e:extrainfo) :=
   let n := lookup_item e.(info) na in
   tRel n.
 
+
 (* In the type definition, (mutual inductive, maybe n different inductive bodies)
    check if the debruijn index [i] refer to a type (being defined),
    if yes, return its reverse order.
@@ -335,7 +320,7 @@ Definition rel_of (na:string) (e:extrainfo) :=
     when we use the function below to check this `nforest`, it should return `Some 0`.
 *)
 Definition is_recursive_call_gen (e:extrainfo) i : option nat:=
-  let l := map (fun x => x.(decl_type)) (lookup_list e.(info) "rels_of_T") in
+  let l := map (fun x => x.(decl_type)) (lookup_list e.(info_source) "rels_of_T") in
   let fix Ffix l j :=
     match l with
     | k :: l0 => if eqb k i then Some j else Ffix l0 (j+1)
@@ -348,14 +333,10 @@ Definition is_recursive_call_gen (e:extrainfo) i : option nat:=
           to the `type term` in the target
 *)
 Definition type_rename_transformer (e:extrainfo) (t:term) : term:=
-  let n_ind := length (lookup_list e.(info) "rels_of_T") in
+  let n_ind := length (lookup_list e.(info_source) "rels_of_T") in
   let fix Ffix e t :=
     match t with
-    | tRel k =>
-      match is_recursive_call_gen e k with
-      | Some i => tInd {| inductive_mind :=e.(kn); inductive_ind := n_ind - i - 1 |} []
-      | None => geti_rename e k
-      end
+    | tRel k => geti_rename e k
     | tApp tx tl => tApp (Ffix e tx) (map (Ffix e) tl)
     | tLambda name t1 t2 => tLambda name (Ffix e t1) (Ffix (update_kp name e NoSave) t2)
     | tProd na t1 t2 => tProd na (Ffix e t1) (Ffix (update_kp na e NoSave) t2)
@@ -363,18 +344,17 @@ Definition type_rename_transformer (e:extrainfo) (t:term) : term:=
   end in
   Ffix e t.
 
-(* Introduce a Prod in the target, introduce a new variable that could be referenced *)
-(* [saveinfo]: if save the information of this new variable into e
-   [na]:       the aname of the new variable
+(* make a Prod term *)
+(* [saveinfo]: if save the information of new variable into e
+   [na]:       the aname of new variable
    [e]:        the local information
-   [t1]:       the type of new variable (need to be fed with extrainfo)
+   [t1]:       the type of new variable
    [t2]:       the term (need to be fed with extrainfo)
 *)
 Definition mktProd (saveinfo:saveinfo) na e (t1:term) (t2:extrainfo -> term) :=
   let e' := update_mk na e saveinfo in
   tProd na (t1) (t2 e').
 
-(* Consume a Prod of the source, introduce it in the target *)
 Definition kptProd (saveinfo:saveinfo) na e (t1:term) (t2:extrainfo -> term) :=
   let e' := update_kp na e saveinfo in
   tProd na (t1) (t2 e').
@@ -396,7 +376,6 @@ Definition it_kptProd (saveinfo:option string) (ctx:context) (e:extrainfo) (t: e
         )
   end in
   Ffix ctx e t.
-
 
 (*iterate mktProd*)
 Definition it_mktProd (saveinfo:option string) (ctx:context) (e:extrainfo) (t: extrainfo -> term) : term :=
@@ -437,13 +416,12 @@ Definition it_mktProd (saveinfo:option string) (ctx:context) (e:extrainfo) (t: e
 *)
 
 
-(* Introduce a Lambda in the target *)
+(* make a Lambda term *)
 Definition mktLambda saveinfo na (e:extrainfo)  (t1:term)
   (t2:extrainfo -> term)
   : term :=
   tLambda na (t1) (t2 (update_mk na e saveinfo)).
 
-(* Consume a Prod of the source, introduce it in the target *)
 Definition kptLambda saveinfo na (e:extrainfo) (t1:term)
   (t2:extrainfo -> term)
   : term :=
@@ -485,8 +463,26 @@ Definition it_kptLambda saveinfo (ctx:context) (e:extrainfo) (t: extrainfo -> te
   end in
   Ffix ctx e t.
 
+(*
+  Used for lambda type argument.
 
-
+  check if a type (_ -> _ -> ... -> ?A) ends with the type that is exactly what we are defining
+  ex. in the definition of Acc,
+      Acc_intro : (forall y : A, R y x -> Acc R y) -> Acc R x.
+      the first argument is a type ends with Acc _ _.
+*)
+Definition check_return_type (t:term) (e:extrainfo) : option nat :=
+  let fix Ffix t e {struct t}:=
+    match t with
+    | tRel i =>
+      let types := lookup_list e.(info_source) "rels_of_T" in
+      let types := map decl_type types in
+      findi i types
+    | tApp t _ => Ffix t e
+    | tProd name _  t2 => Ffix t2 (update_kp name e NoSave)
+    | _ => None
+    end in
+  Ffix t e.
 
 
 (****************************************************************)
@@ -512,62 +508,4 @@ Definition fold_update_kp_util {Y:Type} saveinfo (ctx:context) (e:extrainfo)
   end in
   Ffix ctx e acc.
 
-
-Axiom print_info: extrainfo -> forall {A}, A.
-
-(* Definition skipvar (e:extrainfo) (decl:context_decl): extrainfo :=
-  let item := mkdeclnat decl.(decl_name) None todo in
-  let renaming := item :: (plus_one_index e.(renaming)) in
-  let info := map (
-    fun x => match x with
-    | information_list na l =>
-        if String.eqb na "rels_of_T" then
-          information_list na (plus_one_index l)
-        else x
-    | information_nat na n => x end
-  ) e.(info) in
-  mkinfo renaming info e.(kn). *)
-
-(* try *)
-(*
-Definition update0 (saveinfo:saveinfo) (na:aname) e :extrainfo :=
-  let info := map (
-    fun x => match x with
-    | information_list na l =>
-        if String.eqb na "rels_of_T" then
-          information_list na (plus_one_index l)
-        else x
-    | information_nat na n => information_nat na n end
-  ) e.(info) in
-  let renaming := plus_one_index e.(renaming) in
-  let item := mkdeclnat na None 0 in
-  match saveinfo with
-  | NoSave => mkinfo renaming info e.(kn)
-  | Saveitem str => mkinfo renaming ((information_nat str 0)::info) e.(kn)
-  | Savelist str => mkinfo renaming (replace_add_info info str item) e.(kn)
-  end.
-
-
-Print context.
-
-Definition it_new (saveinfo:saveinfo) (ctx:context) e (t:extrainfo  -> context_decl -> term -> term) (acc:extrainfo -> term) :=
-  let fix Ffix ctx e :=
-    match ctx with
-    | [] => acc e
-    | decl :: ctx' =>
-      let e' := update0 saveinfo decl.(decl_name) e in
-      t e decl (Ffix ctx' e')
-    end in
-  Ffix ctx e. *)
-
-(*
-  it_new (Savelist "params") params initial_info
-    (fun e decl t =>
-      (*
-        if "is uniform param" then tProd _ (type_rename_transformer e decl.(decl_type)) t
-        else
-      *)
-    )
-    (fun e =>
-    )
-*)
+(* Axiom print_info: extrainfo -> forall {A}, A. *)
